Johan Commelin's effort

src/for_mathlib/mv_polynomial.lean
@@ -1,7 +1,14 @@
 import data.mv_polynomial
+import data.polynomial
+
+example : true := trivial -- workaround for the "open_locale at top of file"
+  -- issue
+
+open_locale classical
 
 namespace mv_polynomial
 
+/-- Evaluating the constant polynomial 1 anywhere gives 1 -/
 theorem eval_one {X : Type*} {R : Type*} [comm_semiring R]
   (x : X → R) : eval x 1 = 1 := eval_C _
   
@@ -20,9 +27,138 @@ begin
   rw hd,
 end
 
+end mv_polynomial
+
+namespace polynomial
+
+/-- Over an infinite integral domain a polynomial f is zero if it
+    evaluates to zero everywhere -/
+lemma eval_eq_zero
+  {k : Type*} [integral_domain k] [infinite k] {f : polynomial k}
+  (H : ∀ x, polynomial.eval x f = 0) : f = 0 :=
+begin
+  rcases infinite.exists_not_mem_finset (roots f) with ⟨x, hx⟩,
+  contrapose! hx with hf,
+  rw mem_roots hf,
+  apply H,
+end
+
 /-- Over an infinite integral domain a polynomial f is zero iff it
     evaluates to zero everywhere -/
-lemma mv_polynomial.eval_eq_zero  {k : Type*} [integral_domain k] [infinite k]
+lemma eval_eq_zero_iff
+  {k : Type*} [integral_domain k] [infinite k] {f : polynomial k} :
+  (∀ x, polynomial.eval x f = 0) ↔ f = 0 :=
+⟨polynomial.eval_eq_zero, by { rintro rfl x, exact rfl }⟩
+
+end polynomial
+
+def fin.equiv_empty : fin 0 ≃ empty :=
+{ to_fun := λ i, false.elim $ nat.not_lt_zero _ i.2,
+  inv_fun := empty.elim,
+  left_inv := λ i, false.elim $ nat.not_lt_zero _ i.2,
+  right_inv := λ x, x.elim }
+
+def fin.equiv_pempty : fin 0 ≃ pempty :=
+{ to_fun := λ i, false.elim $ nat.not_lt_zero _ i.2,
+  inv_fun := pempty.elim,
+  left_inv := λ i, false.elim $ nat.not_lt_zero _ i.2,
+  right_inv := λ x, x.elim }
+
+namespace mv_polynomial
+
+@[simp] lemma eval_rename
+  {k : Type*} [comm_semiring k]
+  {m : Type*} {n : Type*} (e : m ≃ n) (f : mv_polynomial m k) (x) :
+  eval x (rename e f) = eval (x ∘ e) f :=
+by apply f.induction_on; { intros, simp * }
+
+lemma equiv_eval_eq_zero
+  {k : Type*} [comm_semiring k]
+  {m : Type*} {n : Type*} (e : m ≃ n)
+  (H : (∀ f : mv_polynomial m k, (∀ x, eval x f = 0) → f = 0))
+  (f : mv_polynomial n k) (hf : ∀ x, eval x f = 0) : f = 0 :=
+begin
+  let φ := ring_equiv_of_equiv k e,
+  suffices h : φ.symm f = 0, { simpa using congr_arg φ h },
+  apply H,
+  intro x,
+  show eval x (rename e.symm f) = 0,
+  simp [hf],
+end
+
+end mv_polynomial
+
+universe variables u v
+
+def equiv.option {X : Type u} {Y : Type v} (e : X ≃ Y) : option X ≃ option Y :=
+{ to_fun := option.map e,
+  inv_fun := option.map e.symm,
+  left_inv := λ x, by { cases x, refl, simp },
+  right_inv :=  λ x, by { cases x, refl, simp } }
+
+def fin_succ_equiv_option (n : ℕ) : fin (n+1) ≃ option (fin n) :=
+sorry
+
+set_option pp.universes true
+
+lemma fintype.induction {P : Π (X : Type*) [fintype X], Prop}
+  (h0 : P pempty) (hs : ∀ (X : Type*) [fintype X], P X → P (option X))
+  (he : ∀ {X Y : Type*} [fintype X] [fintype Y] (e : X ≃ Y), P X → P Y)
+  (X : Type*) [fintype X] : P X :=
+begin
+  rcases fintype.exists_equiv_fin X with ⟨n, ⟨e⟩⟩,
+  apply he (equiv.ulift.trans e.symm), clear e,
+  induction n with n ih,
+  { exact he (equiv.ulift.trans fin.equiv_pempty).symm h0 },
+  { specialize hs _ ih,
+    apply he _ hs,
+    refine (equiv.ulift.trans _).symm,
+    refine (fin_succ_equiv_option n).trans _,
+    refine equiv.ulift.option.symm }
+end
+
+namespace mv_polynomial
+
+/-- Over an infinite integral domain a polynomial f is zero if it
+    evaluates to zero everywhere -/
+lemma fin_eval_eq_zero
+  {k : Type*} [int : integral_domain k] [inf : infinite k]
+  {n : Type*} [fin : fintype n] :
+  ∀ {f : mv_polynomial n k}, (∀ x, eval x f = 0) → f = 0 :=
+begin
+  unfreezeI,
+  revert inf int k,
+  revert fin n,
+  refine fintype.induction _ _ _,
+  { intros k int inf f H,
+    have h : (pempty_ring_equiv k) f = 0 := H _,
+    replace h := congr_arg (pempty_ring_equiv k).symm h,
+    rw [ring_equiv.symm_apply_apply] at h,
+    convert h, symmetry, exact ring_equiv.map_zero _ },
+  { intros n _ ih k int inf f hf,
+    let φ := option_equiv_right k n,
+    suffices h : φ f = 0, { simpa using congr_arg φ.symm h },
+    apply ih,
+    { sorry },
+    { resetI, sorry } },
+  { intros m n _ _ e H k int inf f,
+    apply mv_polynomial.equiv_eval_eq_zero e,
+    apply @H }
+end
+
+/-- Over an infinite integral domain a polynomial f is zero iff it
+    evaluates to zero everywhere -/
+lemma eval_eq_zero_iff
+  {k : Type*} [integral_domain k] [infinite k]
+  {n : Type*} {f : mv_polynomial n k} :
+  (∀ x, eval x f = 0) ↔ f = 0 :=
+begin
+  sorry
+end
+
+/-- Over an infinite integral domain a polynomial f is zero iff it
+    evaluates to zero everywhere -/
+lemma eval_eq_zero  {k : Type*} [integral_domain k] [infinite k]
   {n : Type*} {f : mv_polynomial n k} :
 (∀ x, eval x f = 0) ↔ f = 0 :=
 begin
